Restructure rewriting, valid fragments and lemmas

src/QueryEq.v
@@ -1,4 +1,3 @@
-Require Import List Relations.
 From mathcomp Require Import all_ssreflect.
 Set Implicit Arguments.
 Unset Strict Implicit.
@@ -8,6 +7,8 @@ Set Asymmetric Patterns.
 From Equations Require Import Equations.
 From extructures Require Import ord fset fmap.
 
+
+Require Import SeqExtra.
 
 Require Import Schema.
 Require Import SchemaAux.
@@ -24,525 +25,42 @@ Require Import QueryConformance.
 Require Import QuerySemantic.
 Require Import NRGTNF.
 
-Require Import String.
+Require Import ValidFragments.
+
+Require Import QueryRewrite.
 
 Section Eq.
 
   Variables N Name Vals : ordType.
   Implicit Type schema : @wfSchema Name Vals.
 
-  Inductive Correct schema : (NamedType * NamedType) -> Query -> Prop :=
-  | CF : forall f α root current,
-      query_conforms schema current (SingleField f α) ->
-      Correct schema (root, current) (SingleField f α)
 
-  | CLF : forall l f α root current,
-      query_conforms schema current (LabeledField l f α) ->
-      Correct schema (root, current) (LabeledField l f α)
-               
-  | CNF : forall f α ϕ root current ty',
-      query_conforms schema current (NestedField f α ϕ) ->
-      lookup_field_type schema current f = Some ty' ->
-      Forall (Correct schema (name_of_type ty', name_of_type ty')) ϕ ->
-      Correct schema (root, current) (NestedField f α ϕ) 
-               
-  | CNLF : forall l f α ϕ root current ty',
-      query_conforms schema current (NestedLabeledField l f α ϕ) ->
-      lookup_field_type schema current f = Some ty' ->
-      Forall (Correct schema (name_of_type ty', name_of_type ty')) ϕ ->
-      Correct schema (root, current) (NestedLabeledField l f α ϕ) 
-
-  (* If the query conforms to a type in scope, which is the same as the
-     root type, then anything is correct as the inline's guard 
-     (the conformance check rules out anything weird)
-   *)
-  | CIF_Any : forall root t ϕ,
-      query_conforms schema root (InlineFragment t ϕ) ->
-      Forall (Correct schema (root, t)) ϕ ->
-      Correct schema (root, root) (InlineFragment t ϕ)
-
-  | CIF_Root : forall root current ϕ,
-      query_conforms schema current (InlineFragment root ϕ) ->
-      Forall (Correct schema (root, root)) ϕ ->
-      Correct schema (root, current) (InlineFragment root ϕ)
-
-  (* The inline's guard is the same as the previous one in scope *)            
-  | CIF_Current : forall root current ϕ,
-      (root \in get_possible_types schema current \/ current \in get_possible_types schema root) ->
-      query_conforms schema current (InlineFragment current ϕ) ->
-      Forall (Correct schema (root, current)) ϕ ->
-      Correct schema (root, current) (InlineFragment current ϕ).
-
-
-  Lemma correct_object_E schema root current t ϕ :
-    is_object_type schema t ->
-    Correct schema (root, current) (InlineFragment t ϕ) ->
-    (is_subtype schema (NT t) (NT current)).
-      (*
-    (t = root /\ is_subtype schema (NT t) (NT current)) |
-    (t = current /\ is_subtype schema (NT t) (NT root))]. *)
-  Proof.
-    move=> Hobj Hok.
-    inversion Hok.
-    - move: H2; rewrite /query_conforms.
-      move/and4P=> [_ Hspread _ _].
-      move: (object_spreads_E Hobj Hspread) => [-> | Himpl | Hmb]; rewrite /is_subtype; apply/or3P.
-        by constructor 1; apply/eqP.
-        by constructor 2; rewrite declares_in_implementation.
-        by constructor 3.
-    - move: H2; rewrite /query_conforms.
-      move/and4P=> [_ Hspread _ _].
-      move: (object_spreads_E Hobj Hspread) => [-> | Himpl | Hmb]; rewrite /is_subtype;
-      apply/or3P.                                        
-        by constructor 1; apply/eqP.
-        by constructor 2; rewrite declares_in_implementation.
-        by constructor 3.
-    - by rewrite /is_subtype; apply/or3P; constructor 1; apply/eqP.
-  Qed.
-
-  Lemma correct_conforms schema root current q :
-    Correct schema (root, current) q ->
-    query_conforms schema current q.
-  Proof. by move=> H; inversion H. Qed.
-
-  Lemma queries_correct_conform schema root current queries :
-    Forall (Correct schema (root, current)) queries ->
-    all (query_conforms schema current) queries.
-  Proof.
-    elim: queries => // hd tl IH.
-    move=> H; inversion H => //=.
-    apply/andP; split.
-    apply: (correct_conforms H2).
-    by apply: IH.
-  Qed.
-
-    
-  Definition QueryEq schema (g : @conformedGraph N Name Vals schema) u ty (q1 q2 : Query)  :=
-    query_conforms schema ty q1 ->
-    query_conforms schema ty q2 ->
-    eval schema g u q1 = eval schema g u q2.
-
-  Definition QueriesEq schema (g : @conformedGraph N Name Vals schema) u ty (q1 q2 : seq Query) :=
-    queries_conform schema ty q1 ->
-    queries_conform schema ty q2 ->
-    eval_queries schema g u q1 = eval_queries schema g u q2.
-    
-
-  Lemma inline_nested_empty schema (g : @conformedGraph N Name Vals schema) :
-    forall t1 t2 ϕ,
-      is_object_type schema t1 ->
-      is_object_type schema t2 ->
-      t1 <> t2 ->
-      eval schema g g.(root) (InlineFragment t1 [:: (InlineFragment t2 ϕ)]) = [::].
-  Proof.
-    move=> t1 t2 ϕ.
-    funelim (is_object_type schema t1) => //.
-    funelim (is_object_type schema0 t2) => //.
-    move=> _ _ Hdiff.
-    rewrite eval_equation_5 Heq0.
-    case: eqP => //= <-.
-    rewrite Heq.
-    by case: eqP => // Ht1t2; rewrite Ht1t2 in Hdiff.
-  Qed.
-
-  Lemma inline_query_preserves schema (g : @conformedGraph N Name Vals schema):
-    forall ϕ u,
-      u \in nodes g.(graph) ->
-      eval schema g u ϕ = eval schema g u (InlineFragment u.(type) [:: ϕ]).
-  Proof.
-    move=> ϕ u Hin; case: g Hin.
-    move=> g Hr He Hf Hn /= Hin.
-    rewrite /nodes_have_object_type in Hn.
-    move/seq.allP /(_ u Hin): Hn.
-    case: u Hin => id ty flds Hin. rewrite /type. funelim (is_object_type schema ty) => //.
-    move=> _.
-    rewrite Heq.
-    case: ϕ.
-    move=> name α. rewrite /eval. 
-    simpl.  Admitted.
-
-  Lemma interface_N_obj schema ty :
-    is_interface_type schema ty -> ~~(is_object_type schema ty).
-  Proof. rewrite /is_interface_type.
-    case Hlook: lookup_type => [tdef|] //.
-    case: tdef Hlook => //.
-    rewrite /is_object_type.
-      by move=> i flds Hlook; rewrite Hlook.
-  Qed.
-
-  Lemma inline_preserves_conformance schema type_in_scope ϕ :
-    query_conforms schema type_in_scope ϕ ->
-    query_conforms schema type_in_scope (InlineFragment type_in_scope [:: ϕ]).
-  Proof.
-    rewrite {2}/query_conforms.
-    move=> Hqc.
-    apply/and4P; split=> //.
-    apply/or3P. apply: (type_in_scope_N_scalar_enum Hqc).
-    rewrite /is_fragment_spread_possible /get_possible_types.
-    
-    move: (type_in_scope_N_scalar_enum Hqc) => [Hobj | Hint | Hunion].
-    funelim (is_object_type schema type_in_scope) => //.
-    Admitted.
- 
-  
-  Lemma filter_preserves_pred T (p pred : T -> bool) (s : seq T) :
-    all p s ->
-    all p [seq x <- s | pred x].
-  Proof.
-    elim: s => [//| x s' IH] /=.
-    move/andP=> [Hpx Hall].
-    case (pred x) => //=.
-      by move/IH: Hall => Hall; apply/andP.
-      by apply: IH.
-  Qed.
-
-  
-  Inductive multi {X : Type} (R : relation X) : relation X :=
-  | multi_refl : forall (x : X), multi R x x
-  | multi_step : forall (x y z : X),
-                    R x y ->
-                    multi R y z ->
-                    multi R x z.
-  
-  Inductive QueryRed (schema : @wfSchema Name Vals) (type_in_scope : NamedType) : seq Query -> seq Query -> Prop :=
-
-  | SQ : forall ϕ ϕ',
-      query_conforms schema type_in_scope ϕ ->
-      multi (AtomicQueryRed schema type_in_scope) ϕ ϕ' ->
-      QueryRed schema type_in_scope [:: ϕ] [:: ϕ']
-               
-  | SS1 : forall ϕ ϕ' ϕs ϕs',
-      query_conforms schema type_in_scope ϕ ->
-      all (query_conforms schema type_in_scope) ϕs ->
-      multi (AtomicQueryRed schema type_in_scope) ϕ ϕ' ->
-      multi (QueryRed schema type_in_scope) ϕs ϕs' -> 
-      QueryRed schema type_in_scope (ϕ :: ϕs) (ϕ' :: ϕs')
-                   
-  | SF_None : forall (ϕ : seq (@Query Name Vals)) f α,
-      let ϕ' := filter (fun q => ~~(partial_query_eq (SingleField f α) q)) ϕ in
-      query_conforms schema type_in_scope (SingleField f α) ->
-      all (query_conforms schema type_in_scope) ϕ ->
-      QueryRed schema type_in_scope ((SingleField f α) :: ϕ) ((SingleField f α) :: ϕ')
-
-  | LF_Some : forall (ϕ : seq (@Query Name Vals)) l f α,
-      let ϕ' := filter (fun q => ~~(partial_query_eq (LabeledField l f α) q)) ϕ in
-      query_conforms schema type_in_scope (LabeledField l f α) ->
-      all (query_conforms schema type_in_scope) ϕ ->
-      QueryRed schema type_in_scope ((LabeledField l f α) :: ϕ) ((LabeledField l f α) :: ϕ')
-
-  | NF_Some : forall (ϕ β : seq (@Query Name Vals)) (f : Name) (α α' : {fmap Name -> Vals}),
-      let subqueries := foldr (fun q acc => if q is NestedField f' α' χ then
-                                          if (f' == f) && (α == α') then
-                                            χ ++ acc
-                                          else
-                                            acc
-                                        else
-                                          acc) [::] ϕ
-      in
-      let ϕ' := (filter (fun q => ~~(partial_query_eq (NestedField f α β) q)) ϕ) in
-      query_conforms schema type_in_scope (NestedField f α β) ->
-      all (query_conforms schema type_in_scope) ϕ ->
-      QueryRed schema type_in_scope
-               ((NestedField f α β) :: ϕ)
-               ((NestedField f α (β ++ subqueries)) :: ϕ')
-               
-                
-  | Inline_spread : forall t ϕ ϕ' ϕs,
-      query_conforms schema type_in_scope (InlineFragment t  (ϕ :: ϕ')) ->
-      all (query_conforms schema type_in_scope) ϕs ->
-      QueryRed schema type_in_scope ((InlineFragment t  (ϕ :: ϕ')) :: ϕs)
-                      ((InlineFragment t [:: ϕ]) :: (InlineFragment t ϕ') :: ϕs)
-
-  | Inline_same : forall ϕ,
-      query_conforms schema type_in_scope (InlineFragment type_in_scope ϕ) ->
-      QueryRed schema type_in_scope [:: InlineFragment type_in_scope ϕ] ϕ
-               
-
-  with
-  AtomicQueryRed (schema : @wfSchema Name Vals) (type_in_scope : NamedType) : Query -> Query -> Prop :=
-  | AQR_Refl : forall ϕ,
-      AtomicQueryRed schema type_in_scope ϕ ϕ
-                     
-  | AQR_Nested : forall f α ϕ ϕ' ty',
-      query_conforms schema type_in_scope (NestedField f α ϕ) ->
-      lookup_field_type schema type_in_scope f = Some ty' ->
-      multi (QueryRed schema ty') ϕ ϕ' ->
-      AtomicQueryRed schema type_in_scope (NestedField f α ϕ) (NestedField f α ϕ')
-
-  | AQR_LabeledNested : forall l f α ϕ ϕ' ty',
-      query_conforms schema type_in_scope (NestedLabeledField l f α ϕ) ->
-      lookup_field_type schema type_in_scope f = Some ty' ->
-      multi (QueryRed schema ty') ϕ ϕ' ->
-      AtomicQueryRed schema type_in_scope (NestedLabeledField l f α ϕ) (NestedLabeledField l f α ϕ')
-
-  | AQR_Inline_Wrap : forall ϕ,
-      query_conforms schema type_in_scope ϕ ->
-      AtomicQueryRed schema type_in_scope ϕ (InlineFragment type_in_scope [:: ϕ])
-                     
-  | AQR_Inline : forall t ϕ ϕ',
-      query_conforms schema type_in_scope (InlineFragment t ϕ) ->
-      multi (QueryRed schema t) ϕ ϕ' ->
-      AtomicQueryRed schema type_in_scope (InlineFragment t ϕ) (InlineFragment t ϕ')
-
-  | AQR_Inline_nested : forall t ϕ,
-      query_conforms schema type_in_scope (InlineFragment t [:: InlineFragment t ϕ]) ->
-      AtomicQueryRed schema type_in_scope (InlineFragment t [:: InlineFragment t ϕ]) (InlineFragment t ϕ) 
-
-  | AQR_Inline_Int : forall t ti ϕ,
-      query_conforms schema type_in_scope (InlineFragment ti ϕ) ->
-      t \in implementation schema ti ->
-            AtomicQueryRed schema type_in_scope (InlineFragment ti ϕ) (InlineFragment t ϕ)
-                           
-  | AQR_Inline_Impl : forall ti ϕ,
-      type_in_scope \in implementation schema ti ->
-      query_conforms schema type_in_scope (InlineFragment ti ϕ) ->
-      Forall (Correct schema (type_in_scope, ti)) ϕ ->
-      AtomicQueryRed schema type_in_scope (InlineFragment ti ϕ) (InlineFragment type_in_scope ϕ)
-
-  | AQR_Inline_Member : forall tu ϕ,
-      type_in_scope \in union_members schema tu ->
-      query_conforms schema type_in_scope (InlineFragment tu ϕ) ->
-      Forall (Correct schema (type_in_scope, tu)) ϕ ->
-      AtomicQueryRed schema type_in_scope (InlineFragment tu ϕ) (InlineFragment type_in_scope ϕ)
-                                              
-  .
-
-
-  Lemma asf schema (g : @conformedGraph N Name Vals schema)  u type_in_scope ti ϕ :
-     query_conforms schema type_in_scope (InlineFragment ti ϕ) ->
-     type_in_scope \in implementation schema ti ->
-            eval schema g u (InlineFragment ti ϕ) = eval schema g u (InlineFragment type_in_scope ϕ). 
-  Proof.
-    move=> Hqc Himpl.
-    move: (has_implementation_is_interface Himpl) => Hint.
-    rewrite !eval_equation_5.
-    funelim (is_interface_type schema ti) => //.
-    rewrite Heq.
-    move: (in_implementation_is_object Himpl) => /is_object_type_E [obj [intfs [flds Hlook]]].
-    rewrite Hlook.
-    case: ifP => //.
-    rewrite declares_in_implementation.
-  Abort.
-  (* Missing info on node -> type of node should be same as the one in scope *)
-    
-  
-  (*Lemma AQR_SFE schema ty ϕ n α : AtomicQueryRed schema ty (SingleField n α) ϕ ->
-                               ϕ = SingleField n α.
-  Proof. by move=> H; inversion H. Qed.
-
-  *)
-
-
-  Lemma filter_all_predC1 (T : eqType) (s : seq T) (x : T) :
-    [seq x' <- s | predC1 x x'] = [::] ->
-    forall x', x' \in s -> x' = x.
-    elim: s x => [//| n s' IH] x /=.
-    case: ifP => //.
-    case: eqP => // -> _ /IH H.
-    by move=> x'; rewrite in_cons => /orP [/eqP ->|]; [|apply: H]. 
-  Qed.
-
-
-
-  Lemma queries_conform_cons schema ty hd tl :
-    queries_conform schema ty (hd :: tl) -> query_conforms schema ty hd.
-  Proof.
-    rewrite /queries_conform.
-      by move/andP=> [_ /= /andP [Hhd _]].
-  Qed.
-
-
-  Lemma nested_conforms_list schema ty n α ϕ :
-    query_conforms schema ty (NestedField n α ϕ) -> ϕ != [::].
-  Proof.
-    rewrite /query_conforms.
-    case lookup_field_in_type => // f.
-    case: ifP => // _.
-    by move/and3P=> [Hne _ _].
-  Qed.
-
-  Lemma not_nil_spread {A : eqType} (lst : seq A) : lst != [] -> exists x lst', lst = x :: lst'.
-  Proof.
-      by case: lst => // x lst' H; exists x; exists lst'.  Qed.
-  
-  Lemma single_field_correct schema ty ty' n α :
-    query_conforms schema ty' (SingleField n α) ->
-    Correct schema (ty, ty') (SingleField n α).
-  Proof. by move=> Hqc; apply: CF. Qed.
 
  
 
+  
+ 
 
-  Lemma nf_correct_lookup_some schema root current n α ϕ :
-    Correct schema (root, current) (NestedField n α ϕ) ->
-    exists fld, lookup_field_type schema current n = Some fld. 
-  Proof.
-    move=> H; inversion H.
-      by exists ty'.
-  Qed.
 
-  Lemma nlf_correct_lookup_some schema root current l n α ϕ :
-    Correct schema (root, current) (NestedLabeledField l n α ϕ) ->
-    exists fld, lookup_field_type schema current n = Some fld. 
-  Proof.
-    move=> H; inversion H.
-      by exists ty'.
-  Qed.
 
-  Lemma nf_queries_conform'' schema ty n α ϕ fld :
-    lookup_field_in_type schema ty n = Some fld ->
-    query_conforms schema ty (NestedField n α ϕ) ->
-    queries_conform schema fld.(return_type) ϕ.
-  Proof.
-    move=> Hlook; rewrite /query_conforms.
-    rewrite Hlook.
-    case: ifP => // _; rewrite -/(query_conforms schema fld.(return_type)).
-    move/and3P=> [HNnil Hargs Hall].
-    rewrite /queries_conform.
-    by apply/andP. 
-  Qed.
-
-  Lemma nlf_queries_conform'' schema ty l n α ϕ fld :
-    lookup_field_in_type schema ty n = Some fld ->
-    query_conforms schema ty (NestedLabeledField l n α ϕ) ->
-    queries_conform schema fld.(return_type) ϕ.
-  Proof.
-    move=> Hlook; rewrite /query_conforms.
-    rewrite Hlook.
-    case: ifP => // _; rewrite -/(query_conforms schema fld.(return_type)).
-    move/and3P=> [HNnil Hargs Hall].
-    rewrite /queries_conform.
-    by apply/andP. 
-  Qed.
+ 
+ 
     
-    
-  Lemma lookup_field_or_type schema lookup_type ty name fld :
-    lookup_field_in_type schema lookup_type name = Some fld ->
-    lookup_field_type schema lookup_type name = Some ty ->
-    ty = fld.(return_type).
-  Proof.
-    by rewrite /lookup_field_type; move=> ->; case. Qed.
-
   
-  (**
-     If query is free of issues and its type in the schema is "ty",
-     then its subqueries are also free of issues for the given type.
-   **)
-  Lemma nested_field_subqueries_correct schema root current n α ϕ ty :
-    Correct schema (root, current) (NestedField n α ϕ) ->
-    lookup_field_type schema current n = Some ty ->
-    Forall (Correct schema (name_of_type ty, name_of_type ty)) ϕ.
-  Proof.  by move=> H Hlook; inversion H; rewrite Hlook in H6; case: H6 => ->. Qed.
-
-  Lemma nlf_queries_correct schema root current l n α ϕ fld :
-    lookup_field_type schema current n = Some fld ->
-    Correct schema (root, current) (NestedLabeledField l n α ϕ) ->
-    Forall (Correct schema (name_of_type fld, name_of_type fld)) ϕ.
-  Proof.  by move=> Hlook H; inversion H; rewrite Hlook in H7; case: H7 => ->. Qed.
-  
-
-  Lemma nf_queries_eq schema (g : @conformedGraph N Name Vals schema) u n α ϕ ϕ' :
-    (forall v, eval_queries schema g v ϕ = eval_queries schema g v ϕ') ->
-    eval schema g u (NestedField n α ϕ) = eval schema g u (NestedField n α ϕ').
-  Proof.
-    move=> Hqs.
-    do 2 rewrite eval_equation_3.
-    case lookup_field_type => //.
-    case=> [nt | lt].
-    case get_target_nodes_with_field => // v1 vn /=.
-    by move: (Hqs v1) => ->. 
-    case get_target_nodes_with_field => // v1 vn /=.
-    move: (Hqs v1) => ->.
-  Admitted.
-
-  
-  
-  Lemma u_and_target_nodes_in_nodes (g : @graphQLGraph N Name Vals) u fld :
-    u \in nodes g -> all (fun v => v \in nodes g) (get_target_nodes_with_field g u fld).
-  Proof.
-  Admitted.
-
-  Lemma ohead_in (A : eqType) (lst : seq A) (v : A) :
-    ohead lst = Some v ->
-    v \in lst.
-  Proof.
-    elim: lst => // x lst' IH /=.
-      by case=> ->; rewrite inE; apply/orP; left.
-  Qed.
-    
-  Lemma ohead_in_nodes (g : @graphQLGraph N Name Vals) nds v :
-    all (fun node => node \in nodes g) nds ->
-    ohead nds = Some v ->
-    v \in nodes g. 
-  Proof.
-    elim: nds => // x nds IH /=.
-    by move=> H; case=> Heq; rewrite Heq in H; move/andP: H => [H _]. 
-  Qed.
-
-  Lemma ohead_cons (A : eqType) H (x : A) lst :
-    ohead (x :: lst) = H -> Some x = H.
-  Proof. done. Qed.
-
-  Lemma map_fs {A B C : eqType} (lst : seq A) (f : A -> B -> C) (x y : B):
-    (forall u,
-      u \in lst ->
-            f u x = f u y) ->
-      [seq f v x | v <- lst] = [seq f v y | v <- lst].
-  Proof.
-    elim: lst => // hd lst' IH.
-    move=> H /=. 
-    move: (H hd). rewrite inE. case eqP => // _.
-    move/(_ (orTb (hd \in lst'))) => Hf. rewrite Hf.
-    congr cons.
-    move: H.
-    Admitted.
-
-  Lemma singleton (A : Type) (x y : A) : x = y -> [:: x] = [:: y]. Proof. by move=> ->. Qed.
-
   Lemma nrl_subqueries (n : Name) (ϕ ϕ' : seq (seq (@ResponseObject Name Vals))) : ϕ = ϕ' -> NestedListResult n ϕ = NestedListResult n ϕ'. Proof. by move=> ->. Qed.
 
 
  
-
-  Lemma qwe schema (g : @conformedGraph N Name Vals schema) u qs qs' α n :
-    (forall u : node_eqType N Name Vals, u \in nodes g -> eval_queries schema g u qs = eval_queries schema g u qs') ->
-    [seq (eval_queries schema g v qs) | v <- get_target_nodes_with_field g u {| label := n; args := α |}] =
-  [seq (eval_queries schema g v qs') | v <- get_target_nodes_with_field g u {| label := n; args := α |}].
+  Lemma qwe schema (g : @conformedGraph Name Vals schema) u qs qs' α n :
+    (forall u : node_eqType Name Vals, u \in nodes g -> eval_queries schema g u qs = eval_queries schema g u qs') ->
+    [seq (eval_queries schema g v qs) | v <- neighbours_with_field g u {| label := n; args := α |}] =
+  [seq (eval_queries schema g v qs') | v <- neighbours_with_field g u {| label := n; args := α |}].
   Proof. Admitted.
 
-  Lemma inline_subqueries_conform schema ty t ϕ :
-    query_conforms schema ty (InlineFragment t ϕ) ->
-    queries_conform schema t ϕ.
-  Proof.
-    rewrite /query_conforms.
-    move/and4P=> [_ _ Hne H].
-    by rewrite /queries_conform; apply/andP. 
-  Qed.
+ 
 
-  Lemma inline_subqueries_correct schema root current t ϕ :
-    Correct schema (root, current) (InlineFragment t ϕ) ->
-    Forall (Correct schema (root, t)) ϕ.
-  Proof.
-      by move=> H; inversion H. Qed.
 
-  Lemma no_repeated_filter (ϕ : @Query Name Vals) (ϕ' : seq Query) :
-    ~~(has (partial_query_eq ϕ) (filter (fun q => ~~(partial_query_eq ϕ q)) ϕ')).
-  Proof.
-    elim: ϕ' => // q ϕ' IH.
-    simpl.
-    case: ifP => // Hnpeq.
-    simpl.
-    apply/orP.
-    rewrite /not. move=> [Hpeq | Hhas].
-    move: Hnpeq. rewrite /negb. case: ifP => //. rewrite Hpeq. done.
-    move: IH; rewrite /negb. case: ifP=> //. rewrite Hhas. done.
-  Qed.
-
-  Lemma filter_preserves_non_repeated (ϕ : seq (@Query Name Vals)) p :
-    no_repeated_query ϕ ->
-    no_repeated_query (filter p ϕ).
-  Proof.
-  Admitted.
+ 
 
   Inductive and6 (P1 P2 P3 P4 P5 P6 : Prop) : Prop :=
     And6 of P1 & P2 & P3 & P4 & P5 & P6.
@@ -562,87 +80,19 @@ Section Eq.
       by case b1; case b2; case b3; case b4; case b5; case b6; constructor; try by case.
   Qed.
 
-  Lemma queries_correct_impl schema ty ti queries :
-    ty \in implementation schema ti ->
-    Forall (Correct schema (ty, ti)) queries ->
-    Forall (Correct schema (ty, ty)) queries.
-  Admitted.
-
-  Lemma queries_correct_mb schema ty tu queries :
-    ty \in union_members schema tu ->
-    Forall (Correct schema (ty, tu)) queries ->
-    Forall (Correct schema (ty, ty)) queries.
-  Admitted.     
-
-  Lemma ble schema ty ti queries :
-    ty \in implementation schema ti ->
-    query_conforms schema ty (InlineFragment ti queries) ->
-    Correct schema (ty, ty) (InlineFragment ti queries) ->
-    queries_conform schema ty queries.
-  Admitted.
-
-  Lemma bleble schema ty ti queries :
-    ty \in implementation schema ti ->
-    queries_conform schema ti queries ->
-    Forall (Correct schema (ty, ti)) queries ->
-    queries_conform schema ty queries.
-  Admitted.
-
-  Lemma bleble' schema ty tu queries :
-    ty \in union_members schema tu ->
-    queries_conform schema tu queries ->
-    Forall (Correct schema (ty, tu)) queries ->
-    queries_conform schema ty queries.
-  Admitted.
-
-  Lemma foo schema ty ti queries :
-    is_object_type schema ty ->
-    is_interface_type schema ti ->
-    is_fragment_spread_possible schema ty ti ->
-    queries != [::] ->
-    Forall (Correct schema (ty, ti)) queries ->
-    query_conforms schema ty (InlineFragment ti queries).
-  Proof.
-    move=> Hobj Hint Hspread Hne Hqsok.
-    rewrite /query_conforms.
-    apply/and4P; split=> //.
-      by apply/or3P; constructor 2.
-    by move: (queries_correct_conform Hqsok).
-  Qed.
-
-  Lemma foo' schema ty tu queries :
-    is_object_type schema ty ->
-    is_union_type schema tu ->
-    is_fragment_spread_possible schema ty tu ->
-    queries != [::] ->
-    Forall (Correct schema (ty, tu)) queries ->
-    query_conforms schema ty (InlineFragment tu queries).
-  Proof.
-    move=> Hobj Hunion Hspread Hne Hqsok.
-    rewrite /query_conforms.
-    apply/and4P; split=> //.
-      by apply/or3P; constructor 3.
-    by move: (queries_correct_conform Hqsok).
-  Qed.
   
-  Lemma queries_conform_inv schema ty queries :
-    queries != [::] ->
-    all (query_conforms schema ty) queries ->
-    queries_conform schema ty queries.
-  Proof. by move=> *; rewrite /queries_conform; apply/andP. Qed.
-  
-  Theorem all_q_has_nrgtnf_q schema (g : @conformedGraph N Name Vals schema):
+  Theorem all_q_has_nrgtnf_q schema (g : @conformedGraph Name Vals schema):
     forall (ϕ : @Query Name Vals),
       query_conforms schema schema.(query_type) ϕ ->
       Correct schema (schema.(query_type), schema.(query_type)) ϕ ->
 
       exists (ϕ' : seq (@Query Name Vals)),
-        [/\ ϕ' != [::],
-         Forall (Correct schema (schema.(query_type), schema.(query_type))) ϕ',
+        [/\
+         queries_conform schema schema.(query_type) ϕ',
          are_in_normal_form schema ϕ',
          are_non_redundant ϕ',
-         multi (QueryRed schema schema.(query_type)) [:: ϕ] ϕ' &
-        eval schema g g.(root) ϕ = eval_queries schema g g.(root) ϕ'].
+         multi (QueryRewrite schema schema.(query_type)) [:: ϕ] ϕ' &
+         eval schema g g.(root) ϕ = eval_queries schema g g.(root) ϕ'].
   Proof.
     move=> ϕ.
     elim ϕ using Query_ind with
@@ -652,18 +102,17 @@ Section Eq.
                   Forall (Correct schema (root, current)) qs ->
                   exists (qs' : seq Query),
                     [/\
-                     qs' != [::],
-                     Forall (Correct schema (root, current)) qs',
+                     queries_conform schema current qs',
                      are_in_normal_form schema qs',
                      are_non_redundant qs',
-                     multi (QueryRed schema current) qs qs' &
+                     multi (QueryRewrite schema current) qs qs' &
                      forall u, u \in nodes g -> eval_queries schema g u qs = eval_queries schema g u qs']).
 
     - move=> f α; exists [:: (SingleField f α)]; split => //.
-      by apply: Forall_cons.
+      by rewrite /queries_conform /all; apply/andP; split => //; apply/andP.
       by apply: multi_refl.
     - move=> l f α; exists [:: (LabeledField l f α)]; split => //.
-      by apply: Forall_cons.
+      by rewrite /queries_conform /all; apply/andP; split=> //; apply/andP.
       by apply: multi_refl.              
 
     - move=> f α qs IH Hqc Hok.
@@ -677,20 +126,15 @@ Section Eq.
       move: (nested_field_subqueries_correct Hok Hlook').
       move: Hqsc.
       move: (lookup_field_or_type Hlook Hlook') => Heq; rewrite -Heq => Hqsc Hqsok.
-      move: (IH ty' ty' Hqsc Hqsok) => {IH}; case=> qs' [Hqsne' Hqsok' Hqsnf' Hqsnr' Hred' Hev'].
+      move: (IH ty' ty' Hqsc Hqsok) => {IH}; case=> qs' [Hqsc' Hqsnf' Hqsnr' Hred' Hev'].
       
       exists [:: (NestedField f α qs')]; split => //=.
-      * apply: Forall_cons => //=.
-        apply: CNF => //.
-        move: Hqc.
-        rewrite /query_conforms Hlook.
-        case: ifP => // _.
-        move/and3P=> [_ Hargs _].
-        rewrite /queries_conform -Heq.
+      * rewrite /queries_conform /all; apply/andP; split=> //.
+        rewrite /query_conforms Hlook -/(query_conforms _ _).
+        apply/andP; split=> //.
         apply/and3P; split=> //.
-        apply: (queries_correct_conform Hqsok').
-        apply: Hlook'.
-        apply: Hqsok'.
+        apply/norP.
+        move
       * rewrite /are_in_normal_form.
         apply/andP; split=> //.
         rewrite /all /is_in_normal_form. by apply/andP.
