src/QueryRewrite.v
@@ -1,0 +1,315 @@
+Require Import List Relations.
+
+From mathcomp Require Import all_ssreflect.
+Set Implicit Arguments.
+Unset Strict Implicit.
+Unset Printing Implicit Defensive.
+Set Asymmetric Patterns.
+
+From Equations Require Import Equations.
+
+From extructures Require Import ord fmap.
+
+Require Import Schema.
+Require Import SchemaAux.
+Require Import SchemaWellFormedness.
+Require Import Query.
+Require Import QueryAux.
+Require Import QueryConformance.
+
+Require Import NRGTNF.
+
+Require Import ValidFragments.
+
+Require Import Ssromega.
+
+Section QueryRewrite.
+
+  Variables N Name Vals : ordType.
+  Implicit Type schema : @wfSchema Name Vals.
+
+  Notation is_field := (@QueryAux.is_field Name Vals).
+  Notation is_inline_fragment := (@QueryAux.is_inline_fragment Name Vals).
+  
+  Inductive multi {X : Type} (R : relation X) : relation X :=
+  | multi_refl : forall (x : X), multi R x x
+  | multi_step : forall (x y z : X),
+      R x y ->
+      multi R y z ->
+      multi R x z.
+
+
+  Equations map_In {A B : Type} (l : list A) (f : forall (x : A), In x l -> B) : list B :=
+      map_In nil _ := nil;
+      map_In (cons hd tl) f := cons (f hd _) (map_In (fun x H => f x _)).
+  
+  Lemma map_In_spec {A B : Type} (f : A -> B) (l : list A) :
+    map_In (fun (x : A) (_ : In x l) => f x) = List.map f l.
+  Proof.
+    remember (fun (x : A) (_ : In x l) => f x) as g.
+    funelim (map_In g); rewrite ?H; trivial.
+    Admitted.
+
+
+  Equations β__subqueryextract (filter query: @Query Name Vals) : seq (@Query Name Vals) :=
+    {
+      β__subqueryextract (NestedField f α β) (NestedField f' α' χ) <= (f == f') && (α == α') => {
+          | true => χ;
+          | false => [::]
+      };
+
+      β__subqueryextract (NestedLabeledField l f α β) (NestedLabeledField l' f' α' χ) <= [&& (l == l'), (f == f') & (α == α')] => {
+      | true => χ;
+      | false => [::]
+      };
+
+      β__subqueryextract (InlineFragment t β) (InlineFragment t' χ) <= t == t' => {
+      | true => χ;
+      | false => [::]
+      };
+      
+      β__subqueryextract _ _ := [::]
+    }.
+   
+
+  Equations lift (query : @Query Name Vals) : seq (@Query Name Vals) :=
+    {
+      lift (InlineFragment _ φ) := φ;
+      lift _ := [::]
+    }.
+
+  Equations lift__queries (queries : seq (@Query Name Vals)) : seq (@Query Name Vals) :=
+    {
+      lift__queries [::] := [::];
+      lift__queries (cons hd tl) := (lift hd) ++ (lift__queries tl)
+    }.
+  
+  
+  Equations β__queries (flt : @Query Name Vals) (queries : seq (@Query Name Vals)) : seq (@Query Name Vals) :=
+    {
+      β__queries _ [::] := [::];
+      β__queries flt (cons hd tl) := (β__subqueryextract flt hd) ++ (β__queries flt tl)
+    }.
+
+  
+  Definition γ__φ (flt : Query) (queries : seq Query) : seq (@Query Name Vals) :=
+    [seq query <- queries | ~~ partial_query_eq flt query].
+
+  Obligation Tactic := intros; program_simpl; try ssromega.
+  Equations normalize schema (type_in_scope : @NamedType Name) (queries : seq (@Query Name Vals))  : seq (@Query Name Vals) :=
+    normalize schema type_in_scope queries by rec (queries_size queries) lt :=
+      normalize _ _ [::] := [::];
+      normalize schema type_in_scope (cons (InlineFragment t φ) queries) := 
+          let normalized := normalize schema type_in_scope queries in
+          if t == type_in_scope then
+            normalize schema type_in_scope (φ ++ queries)
+          else
+          if is_subtype schema (NT t) (NT type_in_scope) then
+            (InlineFragment t (normalize schema t φ)) :: normalized
+          else
+            if is_fragment_spread_possible schema type_in_scope t then 
+              normalize schema type_in_scope (φ ++ queries)
+            else
+              (* Should not happen ? *)
+              [::];
+
+            
+      normalize schema type_in_scope (cons query queries) :=
+          let normalized := normalize schema type_in_scope queries in
+          if is_object_type schema type_in_scope then
+              (* In a valid query, if there are fragments, they must be
+                 on supertype or the same type. Then, every field in those
+                 subqueries exist in the current type, therefore they should
+                 be lifted on normalization. *)
+              query :: normalized
+          else
+          if is_interface_type schema type_in_scope then
+            if all is_inline_fragment normalized then
+              map_In (fun q (H : In q normalized) =>
+                        if q is InlineFragment t φ then
+                          InlineFragment t (query :: φ)
+                        else
+                          q)
+            else
+              query :: normalized
+          else
+            [::]
+  .
+  Next Obligation.
+  Qed.
+  Next Obligation.
+  Qed.
+  Next Obligation.
+  Qed.
+  Next Obligation.
+      by rewrite queries_size_app -/(queries_size _); ssromega.
+  Qed.
+  Next Obligation.
+      by rewrite -/(queries_size _); ssromega.
+  Qed.
+  Next Obligation.
+          by rewrite queries_size_app -/(queries_size _); ssromega.
+  Qed.
+
+
+  Lemma normalize_in_object_scope_are_fields schema root current queries :
+    all (has_valid_fragments schema root current) queries ->
+    is_object_type schema current ->
+    all is_field (normalize schema current queries).
+  Proof.
+    funelim (normalize schema current queries) => //.
+    all: do ?[by rewrite {1}/all -/(all _ _) => /andP [Hval Hvals] Hobj; rewrite Hobj;
+              rewrite /all; apply/andP; split => //; apply: (H root)]. 
+
+    rewrite {1}/all -/(all _ _) => /andP [Hval Hvals] Hobj.
+    case: eqP => // Heq.
+    apply: (H0 root).
+    rewrite all_cat; apply/andP; split => //.
+    rewrite Heq in Hval.
+    by apply: (has_valid_fragments_inline_subqueries Hval) => //.
+    exact: Hobj.
+    case: ifP => //.
+    move/(is_subtype_obj_eq Hobj) => Hteq. by rewrite Hteq in Heq.
+    move=> _.
+    case: ifP=> // Hspread.
+    apply: (H0 root) => //.
+    rewrite all_cat; apply/andP; split => //.
+    
+    rewrite has_valid_fragmentsP in Hval.
+
+    
+  Lemma normalize_to_normal_form schema root current queries :
+    all (has_valid_fragments schema root current) queries ->
+    are_in_normal_form schema (normalize schema current queries).
+  Proof.
+    elim: queries root current => // hd tl IH root current.
+    rewrite /all => /andP [Hval Htlval].
+    case: hd Hval.
+    - move=> f α.
+      rewrite normalize_equation_2.
+    rewrite /are_in_normal_form.
+    apply/andP; split.
+    apply/orP. left.
+    simpl.
+    move: (H root Htlval).
+    rewrite /are_in_normal_form.
+
+  
+  Equations normalize schema (type_in_scope : @NamedType Name) (queries : seq (@Query Name Vals)) : seq (@Query Name Vals) :=
+    normalize schema type_in_scope queries by rec (queries_size queries) lt :=
+      normalize schema type_in_scope [::] => [::];
+
+      normalize schema type_in_scope (cons (SingleField f α) ϕ) :=
+        let ϕ' := normalize schema type_in_scope ϕ in
+      
+        if is_object_type schema type_in_scope then
+          let lifted := lift__queries ϕ' in
+          (SingleField f α) :: (γ__φ (SingleField f α) lifted)
+
+        else
+        if is_interface_type schema type_in_scope then
+          let filtered := γ__φ (SingleField f α) ϕ' in
+          map_In (fun query (H : In query filtered) => 
+                     match query with
+                     | InlineFragment t φ => InlineFragment t (normalize schema t ((SingleField f α) :: φ))
+                     | _ => query
+                     end)
+        else
+          (* This should not be possible in a wf query *)
+          [::];
+
+      normalize schema type_in_scope (cons (LabeledField l f α) ϕ) :=
+        let ϕ' := normalize schema type_in_scope ϕ in
+      
+        if is_object_type schema type_in_scope then
+          let lifted := lift__queries ϕ' in
+          (LabeledField l f α) :: (γ__φ (LabeledField l f α) lifted)
+
+        else
+        if is_interface_type schema type_in_scope then
+          let filtered := γ__φ (LabeledField l f α) ϕ' in
+          (map_In (fun query (H : In query filtered) =>
+                     if query is InlineFragment t φ then
+                       InlineFragment t (normalize schema t ((LabeledField l f α) :: φ))
+                     else
+                       query))
+        else
+          (* This should not be possible in a wf query *)
+          [::];
+
+
+      normalize schema type_in_scope (cons (NestedField f α φ) ϕ) :=
+        let ϕ' := normalize schema type_in_scope ϕ in
+
+        if is_object_type schema type_in_scope then
+          let lifted := lift__queries ϕ' in
+          let collected := β__queries (NestedField f α φ) lifted in
+          match lookup_field_type schema type_in_scope f with
+          | Some return_type => (NestedField f α (normalize schema return_type collected)) :: γ__φ (NestedField f α φ) lifted
+          | _ => [::] (* Should never happen *)
+          end
+
+        else
+        if is_interface_type schema type_in_scope then
+          let filtered := γ__φ (NestedField f α φ) ϕ' in
+          map_In (fun query (H : In query filtered) => 
+                    if query is InlineFragment t β then
+                      InlineFragment t (normalize schema t ((NestedField f α φ) :: β))
+                    else
+                      query)
+
+        else
+          (* This should not be possible in a wf query *)
+          [::];
+
+      normalize schema type_in_scope (cons (NestedLabeledField l f α φ) ϕ) :=
+        let ϕ' := normalize schema type_in_scope ϕ in
+
+        if is_object_type schema type_in_scope then
+          let lifted := lift__queries ϕ' in
+          let collected := β__queries (NestedLabeledField l f α φ) lifted in
+          match lookup_field_type schema type_in_scope f with
+          | Some return_type => (NestedLabeledField l f α (normalize schema return_type collected)) :: γ__φ (NestedLabeledField l f α φ) lifted
+          | _ => [::] (* Should never happen *)
+          end
+
+        else
+        if is_interface_type schema type_in_scope then
+          let filtered := γ__φ (NestedLabeledField l f α φ) ϕ' in
+          map_In (fun query (H : In query filtered) =>
+                    if query is InlineFragment t β then
+                      InlineFragment t (normalize schema t ((NestedLabeledField l f α φ) :: β))
+                    else
+                      query)
+
+        else
+          (* This should not be possible in a wf query *)
+          [::];
+
+          
+      normalize schema type_in_scope (cons (InlineFragment t φ) ϕ) :=
+        let ϕ' := normalize schema type_in_scope ϕ in
+
+        if is_object_type schema type_in_scope then
+          normalize schema type_in_scope (φ ++ ϕ')
+        else
+        if is_interface_type schema type_in_scope then
+          if t == type_in_scope then
+            normalize schema type_in_scope (φ ++ ϕ')
+          else (* Object type in valid fragments *)
+            let collected := β__queries (InlineFragment t φ) ϕ' in
+            (InlineFragment t (normalize schema t collected)) :: (γ__φ (InlineFragment t φ) ϕ')        
+      else (* union *)
+        let collected := β__queries (InlineFragment t φ) ϕ' 
+        in
+        (InlineFragment t (normalize schema t collected)) :: (γ__φ (InlineFragment t φ) ϕ')
+  .
+
+  Next Obligation.
+  
+
+
+
+      
+End QueryRewrite.
+
