src/SeqExtra.v
@@ -1,0 +1,72 @@
+
+
+From mathcomp Require Import all_ssreflect.
+Set Implicit Arguments.
+Unset Strict Implicit.
+Unset Printing Implicit Defensive.
+
+
+
+
+
+  Lemma filter_preserves_pred T (p pred : T -> bool) (s : seq T) :
+    all p s ->
+    all p [seq x <- s | pred x].
+  Proof.
+    elim: s => [//| x s' IH] /=.
+    move/andP=> [Hpx Hall].
+    case (pred x) => //=.
+      by move/IH: Hall => Hall; apply/andP.
+      by apply: IH.
+  Qed.
+  
+  Lemma filter_all_predC1 (T : eqType) (s : seq T) (x : T) :
+    [seq x' <- s | predC1 x x'] = [::] ->
+    forall x', x' \in s -> x' = x.
+    elim: s x => [//| n s' IH] x /=.
+    case: ifP => //.
+    case: eqP => // -> _ /IH H.
+    by move=> x'; rewrite in_cons => /orP [/eqP ->|]; [|apply: H]. 
+  Qed.
+
+  
+  Lemma not_nil_spread {A : eqType} (lst : seq A) : lst != [::] -> exists x lst', lst = x :: lst'.
+  Proof.
+      by case: lst => // x lst' H; exists x; exists lst'.  Qed.
+
+  
+
+  Lemma ohead_in (A : eqType) (lst : seq A) (v : A) :
+    ohead lst = Some v ->
+    v \in lst.
+  Proof.
+    elim: lst => // x lst' IH /=.
+      by case=> ->; rewrite inE; apply/orP; left.
+  Qed.
+
+  
+
+  Lemma ohead_cons (A : eqType) H (x : A) lst :
+    ohead (x :: lst) = H -> Some x = H.
+  Proof. done. Qed.
+
+
+  
+
+  Lemma map_fs {A B C : eqType} (lst : seq A) (f : A -> B -> C) (x y : B):
+    (forall u,
+      u \in lst ->
+            f u x = f u y) ->
+      [seq f v x | v <- lst] = [seq f v y | v <- lst].
+  Proof.
+    elim: lst => // hd lst' IH.
+    move=> H /=. 
+    move: (H hd). rewrite inE. case eqP => // _.
+    move/(_ (orTb (hd \in lst'))) => Hf. rewrite Hf.
+    congr cons.
+    move: H.
+  Admitted.
+
+  
+
+  Lemma singleton (A : Type) (x y : A) : x = y -> [:: x] = [:: y]. Proof. by move=> ->. Qed.
