src/ValidFragments.v
@@ -1,0 +1,429 @@
+Require Import List.
+
+From mathcomp Require Import all_ssreflect.
+Set Implicit Arguments.
+Unset Strict Implicit.
+Unset Printing Implicit Defensive.
+Set Asymmetric Patterns.
+
+From extructures Require Import ord fset.
+
+Require Import Schema.
+Require Import SchemaAux.
+Require Import SchemaWellFormedness.
+Require Import Query.
+Require Import QueryConformance.
+
+Require Import NRGTNF.
+
+Section ValidFragments.
+
+  Variables N Name Vals : ordType.
+  Implicit Type schema : @wfSchema Name Vals.
+
+
+  (* Check if it's possible to have an interface fragment in another one :
+     - It is valid to spread an abstract on an abstract as long there is one object type
+       that is a subtype of both -> Check if we eliminate this possibility *)
+  Inductive Correct schema : (NamedType * NamedType) -> Query -> Prop :=
+  | CF : forall f α root current,
+      query_conforms schema current (SingleField f α) ->
+      Correct schema (root, current) (SingleField f α)
+
+  | CLF : forall l f α root current,
+      query_conforms schema current (LabeledField l f α) ->
+      Correct schema (root, current) (LabeledField l f α)
+               
+  | CNF : forall f α ϕ root current ty',
+      query_conforms schema current (NestedField f α ϕ) ->
+      lookup_field_type schema current f = Some ty' ->
+      Forall (Correct schema (tname ty', tname ty')) ϕ ->
+      Correct schema (root, current) (NestedField f α ϕ) 
+               
+  | CNLF : forall l f α ϕ root current ty',
+      query_conforms schema current (NestedLabeledField l f α ϕ) ->
+      lookup_field_type schema current f = Some ty' ->
+      Forall (Correct schema (tname ty', tname ty')) ϕ ->
+      Correct schema (root, current) (NestedLabeledField l f α ϕ) 
+
+  (* If the query conforms to a type in scope, which is the same as the
+     root type, then anything is correct as the inline's guard 
+     (the conformance check rules out anything weird)
+   *)
+  | CIF_Any : forall root t ϕ,
+      t <> root ->
+      query_conforms schema root (InlineFragment t ϕ) ->
+      Forall (Correct schema (root, t)) ϕ ->
+      Correct schema (root, root) (InlineFragment t ϕ)
+
+  | CIF_Root : forall root current ϕ,
+      query_conforms schema current (InlineFragment root ϕ) ->
+      Forall (Correct schema (root, root)) ϕ ->
+      Correct schema (root, current) (InlineFragment root ϕ)
+
+  | CIF_Spread : forall root current t φ,
+      t <> root ->
+      t <> current ->
+      query_conforms schema current (InlineFragment t φ) ->
+      is_fragment_spread_possible schema root t -> 
+      Forall (Correct schema (root, t)) φ ->
+      Correct schema (root, current) (InlineFragment t φ)
+    
+  (*
+    Spec allows fragment to spread in asbtract scopes if there is at least one 
+    object type in both types. This means it is possible to spread again into 
+    this common type.
+   *)
+  | CIF_Subtype : forall root current t φ,
+      query_conforms schema current (InlineFragment t φ) ->
+      Forall (Correct schema (root, t)) φ ->
+      (* An inline fragment cannot "drift" to another type not related to the root one *)
+      is_subtype schema (NT t) (NT root) ->
+      is_subtype schema (NT t) (NT current) ->
+      Correct schema (root, current) (InlineFragment t φ)
+
+        
+  (* The inline's guard is the same as the previous one in scope *)            
+  | CIF_Current : forall root current ϕ,
+      current <> root ->
+      query_conforms schema current (InlineFragment current ϕ) ->
+      Forall (Correct schema (root, current)) ϕ ->
+      Correct schema (root, current) (InlineFragment current ϕ).
+
+
+
+  Fixpoint has_valid_fragments schema (root current : @NamedType Name) query : bool :=
+    query_conforms schema current query &&
+    match query with
+    | NestedField f _ φ => match lookup_field_type schema current f with
+                          | Some return_type => all (has_valid_fragments schema return_type return_type) φ
+                          | _ => false
+                          end
+    | NestedLabeledField _ f _ φ => match lookup_field_type schema current f with
+                                   | Some return_type => all (has_valid_fragments schema return_type return_type) φ
+                                   | _ => false
+                                   end
+    | InlineFragment t φ => if current == root then
+                             if t != root then
+                               (* CIF_Any *)
+                               all (has_valid_fragments schema root t) φ
+                             else
+                               (* CIF_Root with current = root *)
+                               all (has_valid_fragments schema root root) φ
+                           else
+                             if t == root then
+                               (* CIF_Root with current ≠ root *)
+                               all (has_valid_fragments schema root root) φ
+                             else
+                             if t == current then
+                               (* CIF_Current *)
+                               all (has_valid_fragments schema root current) φ
+                             else
+                             if is_subtype schema (NT t) (NT root) && is_subtype schema (NT t) (NT current) then
+                               (* CIF Subtype *)
+                               all (has_valid_fragments schema root t) φ
+                             else
+                             if is_fragment_spread_possible schema root t then
+                               (* CIF_Spread *)
+                               all (has_valid_fragments schema root t) φ
+                             else
+                               false
+    | _ => true
+    
+    end.
+
+
+  Lemma valid_fragmentsP schema root current query :
+    reflect (Correct schema (root, current) query)
+            (has_valid_fragments schema root current query).
+  Proof.
+    apply: (iffP idP).
+    - move: schema root current.
+      elim query using Query_ind with
+          (Pl := fun (qs : seq Query) =>
+                  forall schema root current,
+                  (all (has_valid_fragments schema root current) qs) ->
+                  (Forall (Correct schema (root, current)) qs)) => //.
+      * move=> f α schema root current; rewrite /has_valid_fragments => /andP [H _].
+          by constructor.
+      * move=> l f α schema root current; rewrite /has_valid_fragments => /andP [H _].
+          by constructor.
+      * move=> f α φ IH schema root current.
+        rewrite /has_valid_fragments => /andP [H].
+        case Hlook: lookup_field_type =>[rty|] //.
+        rewrite -/(has_valid_fragments _ _ _).
+        move/(IH schema rty rty) => Hall.
+          by apply: CNF; [| apply: Hlook |].
+      * move=> l f α φ IH schema root current.
+        rewrite /has_valid_fragments => /andP [H].
+        case Hlook: lookup_field_type =>[rty|] //.
+        rewrite -/(has_valid_fragments _ _ _).
+        move/(IH schema rty rty) => Hall.
+          by apply: CNLF; [| apply: Hlook |].
+      * move=> t φ IH schema root current.
+        rewrite /has_valid_fragments => /andP [Hqc].
+        case: ifP => //.
+        move=> /eqP Heq.
+        case: ifP => // Hneq.
+        move/(IH schema root t) => Hall.
+        rewrite Heq in Hqc *.
+        by apply: CIF_Any => //; apply/eqP.
+        move/eqP: Hneq => Heqt.
+        move/(IH schema root root)=> Hall.
+        rewrite Heqt in Hqc *.
+        by apply: CIF_Root => //.
+        move/eqP=> Hneq.
+        case: ifP => // /eqP Heqt.
+        move/(IH schema root root)=> Hall.
+        rewrite Heqt in Hqc *.
+        by apply: CIF_Root => //.
+        case: ifP => // /eqP Heq.
+        move/(IH schema root current) => Hall.
+        rewrite Heq in Hqc *.
+        by apply: CIF_Current; rewrite Heq in Heqt.
+        case: ifP => // /andP.
+        case=> [Hsubroot Hsubcurr].
+        move/(IH schema root t)=> Hall.
+        by apply: CIF_Subtype.
+        move=> _.
+        case: ifP => // Hspread.
+        move/(IH schema root t)=> Hall.
+          by apply: CIF_Spread.
+      * move=> hd IH tl IH' schema root current.
+        rewrite /all => /andP [Hval Htlval].
+        apply/Forall_cons.
+            by apply: (IH schema root current Hval).
+            by apply: (IH' schema root current Htlval).
+    - move: schema root current.
+      elim query using Query_ind with
+          (Pl := fun qs =>
+                  forall schema root current,
+                  Forall (Correct schema (root, current)) qs ->
+                  all (has_valid_fragments schema root current) qs) => //.
+      * by intros; inversion H; rewrite /has_valid_fragments; apply/andP.
+      * by intros; inversion H; rewrite /has_valid_fragments; apply/andP.
+      * move=> f α φ IH schema root current Hc; inversion Hc.
+        rewrite /has_valid_fragments; apply/andP; split => //.
+        by rewrite H5; apply: (IH schema ty' ty' H6).
+      * move=> l f α φ IH schema root current Hc; inversion Hc.
+        rewrite /has_valid_fragments; apply/andP; split => //.
+          by rewrite H6; apply: (IH schema ty' ty' H7).
+      * move=> t φ IH schema root current Hc; inversion Hc.
+        + rewrite /has_valid_fragments; apply/andP; split => //.
+          case: ifP => // _.
+          case: ifP => // /eqP Hneq.
+            by apply: (IH schema current t H5).
+            by rewrite Hneq in H5; apply: (IH schema current current  H5).
+          case: ifP => // /eqP Heq.
+            by rewrite Heq in H5; apply: (IH schema current current H5). 
+          case: eqP => // _.
+
+  Admitted.
+
+  Lemma has_valid_fragments_inline_subqueries schema root current t φ :
+    has_valid_fragments schema root current (InlineFragment t φ) ->
+    all (has_valid_fragments schema root t) φ.
+  Proof.
+    rewrite /has_valid_fragments => /andP [Hqc].
+    case: eqP => // Heq.
+    case: eqP => // Hneq /=.
+      by rewrite Hneq.
+      case: eqP => //= Hteq.
+      by rewrite Hteq.
+    case: eqP => // Hteq'. by rewrite Hteq'.
+    case: ifP => // _.
+    case: ifP => //.
+  Qed.
+
+ 
+    
+  Lemma correct_object_E schema root current t ϕ :
+    is_object_type schema t ->
+    Correct schema (root, current) (InlineFragment t ϕ) ->
+    (is_subtype schema (NT t) (NT current)).
+      (*
+    (t = root /\ is_subtype schema (NT t) (NT current)) |
+    (t = current /\ is_subtype schema (NT t) (NT root))]. *)
+  Proof.
+    move=> Hobj Hok.
+    inversion Hok => //.
+    - move: H4; rewrite /query_conforms.
+      move/and4P=> [_ Hspread _ _].
+      move: (object_spreads_E Hobj Hspread) => [-> | Himpl | Hmb]; rewrite /is_subtype; apply/or3P.
+        by constructor 1; apply/eqP.
+        by constructor 2; rewrite declares_in_implementation.
+        by constructor 3.
+    - move: H2; rewrite /query_conforms.
+      move/and4P=> [_ Hspread _ _].
+      move: (object_spreads_E Hobj Hspread) => [-> | Himpl | Hmb]; rewrite /is_subtype;
+      apply/or3P.                                        
+        by constructor 1; apply/eqP.
+        by constructor 2; rewrite declares_in_implementation.
+        by constructor 3.
+  Abort.
+
+  Lemma correct_conforms schema root current q :
+    Correct schema (root, current) q ->
+    query_conforms schema current q.
+  Proof. by move=> H; inversion H. Qed.
+
+  Lemma queries_correct_conform schema root current queries :
+    Forall (Correct schema (root, current)) queries ->
+    all (query_conforms schema current) queries.
+  Proof.
+    elim: queries => // hd tl IH.
+    move=> H; inversion H => //=.
+    apply/andP; split.
+    apply: (correct_conforms H2).
+    by apply: IH.
+  Qed.
+
+   Lemma single_field_correct schema ty ty' n α :
+    query_conforms schema ty' (SingleField n α) ->
+    Correct schema (ty, ty') (SingleField n α).
+  Proof. by move=> Hqc; apply: CF. Qed.
+
+ 
+
+
+  Lemma nf_correct_lookup_some schema root current n α ϕ :
+    Correct schema (root, current) (NestedField n α ϕ) ->
+    exists fld, lookup_field_type schema current n = Some fld. 
+  Proof.
+    move=> H; inversion H.
+      by exists ty'.
+  Qed.
+
+  Lemma nlf_correct_lookup_some schema root current l n α ϕ :
+    Correct schema (root, current) (NestedLabeledField l n α ϕ) ->
+    exists fld, lookup_field_type schema current n = Some fld. 
+  Proof.
+    move=> H; inversion H.
+      by exists ty'.
+  Qed.
+
+  Lemma nf_queries_conform'' schema ty n α ϕ fld :
+    lookup_field_in_type schema ty n = Some fld ->
+    query_conforms schema ty (NestedField n α ϕ) ->
+    queries_conform schema fld.(return_type) ϕ.
+  Proof.
+    move=> Hlook; rewrite /query_conforms.
+    rewrite Hlook.
+    rewrite -/(query_conforms schema fld.(return_type)).
+    move/and4P=> [Hnty HNnil Hargs Hall].
+    rewrite /queries_conform.
+    by apply/andP. 
+  Qed.
+
+  Lemma nlf_queries_conform'' schema ty l n α ϕ fld :
+    lookup_field_in_type schema ty n = Some fld ->
+    query_conforms schema ty (NestedLabeledField l n α ϕ) ->
+    queries_conform schema fld.(return_type) ϕ.
+  Proof.
+    move=> Hlook; rewrite /query_conforms.
+    rewrite Hlook -/(query_conforms schema fld.(return_type)).
+    move/and4P=> [Hnty HNnil Hargs Hall].
+    rewrite /queries_conform.
+    by apply/andP. 
+  Qed.
+
+  
+  
+  (**
+     If query is free of issues and its type in the schema is "ty",
+     then its subqueries are also free of issues for the given type.
+   **)
+  Lemma nested_field_subqueries_correct schema root current n α ϕ ty :
+    Correct schema (root, current) (NestedField n α ϕ) ->
+    lookup_field_type schema current n = Some ty ->
+    Forall (Correct schema (tname ty, tname ty)) ϕ.
+  Proof.  by move=> H Hlook; inversion H; rewrite Hlook in H6; case: H6 => ->. Qed.
+
+  Lemma nlf_queries_correct schema root current l n α ϕ fld :
+    lookup_field_type schema current n = Some fld ->
+    Correct schema (root, current) (NestedLabeledField l n α ϕ) ->
+    Forall (Correct schema (tname fld, tname fld)) ϕ.
+  Proof.  by move=> Hlook H; inversion H; rewrite Hlook in H7; case: H7 => ->. Qed.
+
+  
+  Lemma inline_subqueries_correct schema root current t ϕ :
+    Correct schema (root, current) (InlineFragment t ϕ) ->
+    Forall (Correct schema (root, t)) ϕ.
+  Proof.
+      by move=> H; inversion H. Qed.
+
+
+  
+  Lemma queries_correct_impl schema ty ti queries :
+    ty \in implementation schema ti ->
+    Forall (Correct schema (ty, ti)) queries ->
+    Forall (Correct schema (ty, ty)) queries.
+  Admitted.
+
+  Lemma queries_correct_mb schema ty tu queries :
+    ty \in union_members schema tu ->
+    Forall (Correct schema (ty, tu)) queries ->
+    Forall (Correct schema (ty, ty)) queries.
+  Admitted.     
+
+  Lemma ble schema ty ti queries :
+    ty \in implementation schema ti ->
+    query_conforms schema ty (InlineFragment ti queries) ->
+    Correct schema (ty, ty) (InlineFragment ti queries) ->
+    queries_conform schema ty queries.
+  Admitted.
+
+  Lemma bleble schema ty ti queries :
+    ty \in implementation schema ti ->
+    queries_conform schema ti queries ->
+    Forall (Correct schema (ty, ti)) queries ->
+    queries_conform schema ty queries.
+  Admitted.
+
+  Lemma bleble' schema ty tu queries :
+    ty \in union_members schema tu ->
+    queries_conform schema tu queries ->
+    Forall (Correct schema (ty, tu)) queries ->
+    queries_conform schema ty queries.
+  Admitted.
+
+  
+
+  Lemma foo schema ty ti queries :
+    is_object_type schema ty ->
+    is_interface_type schema ti ->
+    is_fragment_spread_possible schema ty ti ->
+    queries != [::] ->
+    Forall (Correct schema (ty, ti)) queries ->
+    query_conforms schema ty (InlineFragment ti queries).
+  Proof.
+    move=> Hobj Hint Hspread Hne Hqsok.
+    rewrite /query_conforms.
+    apply/and4P; split=> //.
+      by apply/or3P; constructor 2.
+    by move: (queries_correct_conform Hqsok).
+  Qed.
+
+  Lemma foo' schema ty tu queries :
+    is_object_type schema ty ->
+    is_union_type schema tu ->
+    is_fragment_spread_possible schema ty tu ->
+    queries != [::] ->
+    Forall (Correct schema (ty, tu)) queries ->
+    query_conforms schema ty (InlineFragment tu queries).
+  Proof.
+    move=> Hobj Hunion Hspread Hne Hqsok.
+    rewrite /query_conforms.
+    apply/and4P; split=> //.
+      by apply/or3P; constructor 3.
+    by move: (queries_correct_conform Hqsok).
+  Qed.
+
+
+  Lemma normalized_queries_are_valid schema type_in_scope φ :
+    is_in_normal_form schema φ ->
+    query_conforms schema type_in_scope φ ->
+    Correct schema (type_in_scope, type_in_scope) φ.
+  Abort.
+
+End ValidFragments.
